Simplify constructor contexts

theories/tree.v
@@ -28,53 +28,32 @@ Inductive zipper : Set :=
 
 (* Top-down *)
 
-Inductive ctx0 : Set :=
-| Node0 (z : ctx0) (x : Z) (r : tree)
-| Node2 (l : tree) (x : Z) (z : ctx0)
-| Node0' (* Hole *) (x : Z) (r : tree)
-| Node2' (l : tree) (x : Z) (* Hole *).
-
 Inductive ctx : Set :=
-| Ctx0 (z : ctx0)
-| Hole.
+| Hole
+| Node0 (l : ctx) (x : Z) (r : tree)
+| Node2 (l : tree) (x : Z) (r : ctx).
 
-Fixpoint comp0 (z1 z2 : ctx0) : ctx0 :=
+Fixpoint comp (z1 : ctx) (z2 : ctx) :=
   match z1 with
-  | Node0 zl x r => Node0 (comp0 zl z2) x r
-  | Node2 l x zr => Node2 l x (comp0 zr z2)
-  | Node0' x r => Node0 z2 x r
-  | Node2' l x => Node2 l x z2 
-  end.
-
-Definition comp' (z1 : ctx) (z2 : ctx0) : ctx0 :=
-  match z1 with
-  | Ctx0 z1 => comp0 z1 z2
+  | Node0 zl x r => Node0 (comp zl z2) x r
+  | Node2 l x zr => Node2 l x (comp zr z2)
   | Hole => z2
   end.
 
-Definition comp (z1 : ctx) (z2 : ctx0) : ctx :=
-  Ctx0 (comp' z1 z2).
-
-Fixpoint plug0 (z : ctx0) (t : tree) : tree :=
+Fixpoint plug (z : ctx) (t : tree) : tree :=
   match z with
-  | Node0 zl x r => Node (plug0 zl t) x r
-  | Node2 l x zr => Node l x (plug0 zr t)
-  | Node0' x r => Node t x r
-  | Node2' l x => Node l x t
-  end.
-
-Definition plug (z : ctx) (t : tree) : tree :=
-  match z with
-  | Ctx0 z => plug0 z t
+  | Node0 zl x r => Node (plug zl t) x r
+  | Node2 l x zr => Node l x (plug zr t)
   | Hole => t
   end.
 
 (* Context laws *)
 
-Lemma comp_plug (z : ctx) (z' : ctx0) (t : tree)
-  : plug (comp z z') t = plug z (plug (Ctx0 z') t).
+Lemma comp_plug (z1 : ctx) (z2 : ctx) (t : tree)
+  : plug (comp z1 z2) t = plug z1 (plug z2 t).
 Proof.
-    destruct z.
-    - induction z; simpl; try (unfold plug, comp in IHz; rewrite IHz); done.
-    - unfold plug, comp; done.
+  induction z1.
+  - simpl; done.
+  - simpl; rewrite IHz1; done.
+  - simpl; rewrite IHz1; done.
 Qed.
